Batteries/Data/RBMap/Lemmas.lean
@@ -11,6 +11,8 @@ public import Batteries.Data.List.Lemmas
 
 @[expose] public section
 
+set_option linter.deprecated false
+
 /-!
 # Additional lemmas for Red-black trees
 -/
@@ -21,33 +23,43 @@ open RBColor
 
 attribute [simp] fold foldl foldr Any forM foldlM Ordered
 
-@[simp] theorem min?_reverse (t : RBNode α) : t.reverse.min? = t.max? := by
+@[deprecated "Use `Std.TreeMap` instead." (since := "2026-05-05"), simp]
+theorem min?_reverse (t : RBNode α) : t.reverse.min? = t.max? := by
   unfold RBNode.max?; split <;> simp [RBNode.min?]
   unfold RBNode.min?; rw [min?.match_1.eq_3]
   · apply min?_reverse
   · simpa [reverse_eq_iff]
 
-@[simp] theorem max?_reverse (t : RBNode α) : t.reverse.max? = t.min? := by
+@[deprecated "Use `Std.TreeMap` instead." (since := "2026-05-05"), simp]
+theorem max?_reverse (t : RBNode α) : t.reverse.max? = t.min? := by
   rw [← min?_reverse, reverse_reverse]
 
-@[simp] theorem mem_nil {x} : ¬x ∈ (.nil : RBNode α) := by simp [Membership.mem, EMem]
-@[simp] theorem mem_node {y c a x b} :
+@[deprecated "Use `Std.TreeMap` instead." (since := "2026-05-05"), simp]
+theorem mem_nil {x} : ¬x ∈ (.nil : RBNode α) := by simp [Membership.mem, EMem]
+@[deprecated "Use `Std.TreeMap` instead." (since := "2026-05-05"), simp]
+theorem mem_node {y c a x b} :
     y ∈ (.node c a x b : RBNode α) ↔ y = x ∨ y ∈ a ∨ y ∈ b := by simp [Membership.mem, EMem]
 
+@[deprecated "Use `Std.TreeMap` instead." (since := "2026-05-05")]
 theorem All_def {t : RBNode α} : t.All p ↔ ∀ x ∈ t, p x := by
   induction t <;> simp [or_imp, forall_and, *]
 
+@[deprecated "Use `Std.TreeMap` instead." (since := "2026-05-05")]
 theorem Any_def {t : RBNode α} : t.Any p ↔ ∃ x ∈ t, p x := by
   induction t <;> simp [or_and_right, exists_or, *]
 
+@[deprecated "Use `Std.TreeMap` instead." (since := "2026-05-05")]
 theorem memP_def : MemP cut t ↔ ∃ x ∈ t, cut x = .eq := Any_def
 
+@[deprecated "Use `Std.TreeMap` instead." (since := "2026-05-05")]
 theorem mem_def : Mem cmp x t ↔ ∃ y ∈ t, cmp x y = .eq := Any_def
 
+@[deprecated "Use `Std.TreeMap` instead." (since := "2026-05-05")]
 theorem mem_congr [Std.TransCmp (α := α) cmp] {t : RBNode α} (h : cmp x y = .eq) :
     Mem cmp x t ↔ Mem cmp y t := by
   rw [Mem, Mem, iff_iff_eq]; congr 1; funext; rw [Std.TransCmp.congr_left h]
 
+@[deprecated "Use `Std.TreeMap` instead." (since := "2026-05-05")]
 theorem isOrdered_iff' [Std.TransCmp (α := α) cmp] {t : RBNode α} :
     isOrdered cmp t L R ↔
     (∀ a ∈ L, t.All (cmpLT cmp a ·)) ∧
@@ -70,9 +82,11 @@ theorem isOrdered_iff' [Std.TransCmp (α := α) cmp] {t : RBNode α} :
         ⟨fun _ h => (hL _ h).2.1, lv, fun _ h => (hL _ h).1, ol⟩,
         ⟨vr, fun _ h => (hR _ h).2.2, fun _ h => (hR _ h).1, or⟩⟩⟩
 
+@[deprecated "Use `Std.TreeMap` instead." (since := "2026-05-05")]
 theorem isOrdered_iff [Std.TransCmp (α := α) cmp] {t : RBNode α} :
     isOrdered cmp t ↔ Ordered cmp t := by simp [isOrdered_iff']
 
+@[deprecated "Use `Std.TreeMap` instead." (since := "2026-05-05")]
 instance (cmp) [Std.TransCmp (α := α) cmp] (t) : Decidable (Ordered cmp t) :=
   decidable_of_iff _ isOrdered_iff
 
@@ -82,20 +96,24 @@ but it can make things that are distinguished by `cmp` equal.
 This is sufficient for `find?` to locate an element on which `cut` returns `.eq`,
 but there may be other elements, not returned by `find?`, on which `cut` also returns `.eq`.
 -/
+@[deprecated "Use `Std.TreeMap` instead." (since := "2026-05-05")]
 class IsCut (cmp : α → α → Ordering) (cut : α → Ordering) : Prop where
   /-- The set `{x | cut x = .lt}` is downward-closed. -/
   le_lt_trans [Std.TransCmp cmp] : cmp x y ≠ .gt → cut x = .lt → cut y = .lt
   /-- The set `{x | cut x = .gt}` is upward-closed. -/
   le_gt_trans [Std.TransCmp cmp] : cmp x y ≠ .gt → cut y = .gt → cut x = .gt
 
+@[deprecated "Use `Std.TreeMap` instead." (since := "2026-05-05")]
 theorem IsCut.lt_trans [IsCut cmp cut] [Std.TransCmp cmp]
     (H : cmp x y = .lt) : cut x = .lt → cut y = .lt :=
   IsCut.le_lt_trans <| Std.OrientedCmp.not_gt_of_gt <| Std.OrientedCmp.gt_iff_lt.2 H
 
+@[deprecated "Use `Std.TreeMap` instead." (since := "2026-05-05")]
 theorem IsCut.gt_trans [IsCut cmp cut] [Std.TransCmp cmp]
     (H : cmp x y = .lt) : cut y = .gt → cut x = .gt :=
   IsCut.le_gt_trans <| Std.OrientedCmp.not_gt_of_gt <| Std.OrientedCmp.gt_iff_lt.2 H
 
+@[deprecated "Use `Std.TreeMap` instead." (since := "2026-05-05")]
 theorem IsCut.congr [IsCut cmp cut] [Std.TransCmp cmp] (H : cmp x y = .eq) :
     cut x = cut y := by
   cases ey : cut y
@@ -107,6 +125,7 @@ theorem IsCut.congr [IsCut cmp cut] [Std.TransCmp cmp] (H : cmp x y = .eq) :
       cases H.symm.trans <| Std.OrientedCmp.gt_iff_lt.1 h
   · exact IsCut.le_gt_trans (fun h => nomatch H.symm.trans h) ey
 
+@[deprecated "Use `Std.TreeMap` instead." (since := "2026-05-05")]
 instance (cmp cut) [@IsCut α cmp cut] : IsCut (flip cmp) (cut · |>.swap) where
   le_lt_trans h₁ h₂ := by
     have : Std.TransCmp cmp := inferInstanceAs (Std.TransCmp (flip (flip cmp)))
@@ -119,16 +138,19 @@ instance (cmp cut) [@IsCut α cmp cut] : IsCut (flip cmp) (cut · |>.swap) where
 `IsStrictCut` upgrades the `IsCut` property to ensure that at most one element of the tree
 can match the cut, and hence `find?` will return the unique such element if one exists.
 -/
+@[deprecated "Use `Std.TreeMap` instead." (since := "2026-05-05")]
 class IsStrictCut (cmp : α → α → Ordering) (cut : α → Ordering) : Prop extends IsCut cmp cut where
   /-- If `cut = x`, then `cut` and `x` have compare the same with respect to other elements. -/
   exact [Std.TransCmp cmp] : cut x = .eq → cmp x y = cut y
 
 /-- A "representable cut" is one generated by `cmp a` for some `a`. This is always a valid cut. -/
+@[deprecated "Use `Std.TreeMap` instead." (since := "2026-05-05")]
 instance (cmp) (a : α) : IsStrictCut cmp (cmp a) where
   le_lt_trans h₁ h₂ := Std.TransCmp.lt_of_lt_of_le h₂ h₁
   le_gt_trans h₁ := Decidable.not_imp_not.1 (Std.TransCmp.le_trans · h₁)
   exact h := (Std.TransCmp.congr_left h).symm
 
+@[deprecated "Use `Std.TreeMap` instead." (since := "2026-05-05")]
 instance (cmp cut) [@IsStrictCut α cmp cut] : IsStrictCut (flip cmp) (cut · |>.swap) where
   exact h := by
     have : Std.TransCmp cmp := inferInstanceAs (Std.TransCmp (flip (flip cmp)))
@@ -136,60 +158,76 @@ instance (cmp cut) [@IsStrictCut α cmp cut] : IsStrictCut (flip cmp) (cut · |>
 
 section fold
 
+@[deprecated "Use `Std.TreeMap` instead." (since := "2026-05-05")]
 theorem foldr_cons (t : RBNode α) (l) : t.foldr (·::·) l = t.toList ++ l := by
   unfold toList
   induction t generalizing l with
   | nil => rfl
   | node _ a _ b iha ihb => rw [foldr, foldr, iha, iha (_::_), ihb]; simp
 
-@[simp] theorem toList_nil : (.nil : RBNode α).toList = [] := rfl
+@[deprecated "Use `Std.TreeMap` instead." (since := "2026-05-05"), simp]
+theorem toList_nil : (.nil : RBNode α).toList = [] := rfl
 
-@[simp] theorem toList_node : (.node c a x b : RBNode α).toList = a.toList ++ x :: b.toList := by
+@[deprecated "Use `Std.TreeMap` instead." (since := "2026-05-05"), simp]
+theorem toList_node : (.node c a x b : RBNode α).toList = a.toList ++ x :: b.toList := by
   rw [toList, foldr, foldr_cons]; rfl
 
-@[simp] theorem toList_reverse (t : RBNode α) : t.reverse.toList = t.toList.reverse := by
+@[deprecated "Use `Std.TreeMap` instead." (since := "2026-05-05"), simp]
+theorem toList_reverse (t : RBNode α) : t.reverse.toList = t.toList.reverse := by
   induction t <;> simp [*]
 
-@[simp] theorem mem_toList {t : RBNode α} : x ∈ t.toList ↔ x ∈ t := by
+@[deprecated "Use `Std.TreeMap` instead." (since := "2026-05-05"), simp]
+theorem mem_toList {t : RBNode α} : x ∈ t.toList ↔ x ∈ t := by
   induction t <;> simp [*, or_left_comm]
 
-@[simp] theorem mem_reverse {t : RBNode α} : a ∈ t.reverse ↔ a ∈ t := by rw [← mem_toList]; simp
+@[deprecated "Use `Std.TreeMap` instead." (since := "2026-05-05"), simp]
+theorem mem_reverse {t : RBNode α} : a ∈ t.reverse ↔ a ∈ t := by rw [← mem_toList]; simp
 
+@[deprecated "Use `Std.TreeMap` instead." (since := "2026-05-05")]
 theorem min?_eq_toList_head? {t : RBNode α} : t.min? = t.toList.head? := by
   induction t with
   | nil => rfl
   | node _ l _ _ ih =>
     cases l <;> simp [RBNode.min?, ih]
 
+@[deprecated "Use `Std.TreeMap` instead." (since := "2026-05-05")]
 theorem max?_eq_toList_getLast? {t : RBNode α} : t.max? = t.toList.getLast? := by
   rw [← min?_reverse, min?_eq_toList_head?]; simp
 
+@[deprecated "Use `Std.TreeMap` instead." (since := "2026-05-05")]
 theorem foldr_eq_foldr_toList {t : RBNode α} : t.foldr f init = t.toList.foldr f init := by
   induction t generalizing init <;> simp [*]
 
+@[deprecated "Use `Std.TreeMap` instead." (since := "2026-05-05")]
 theorem foldl_eq_foldl_toList {t : RBNode α} : t.foldl f init = t.toList.foldl f init := by
   induction t generalizing init <;> simp [*]
 
+@[deprecated "Use `Std.TreeMap` instead." (since := "2026-05-05")]
 theorem foldl_reverse {α β : Type _} {t : RBNode α} {f : β → α → β} {init : β} :
     t.reverse.foldl f init = t.foldr (flip f) init := by
   simp (config := {unfoldPartialApp := true})
     [foldr_eq_foldr_toList, foldl_eq_foldl_toList, flip]
 
+@[deprecated "Use `Std.TreeMap` instead." (since := "2026-05-05")]
 theorem foldr_reverse {α β : Type _} {t : RBNode α} {f : α → β → β} {init : β} :
     t.reverse.foldr f init = t.foldl (flip f) init :=
   foldl_reverse.symm.trans (by simp; rfl)
 
+@[deprecated "Use `Std.TreeMap` instead." (since := "2026-05-05")]
 theorem forM_eq_forM_toList [Monad m] [LawfulMonad m] {t : RBNode α} :
     t.forM (m := m) f = t.toList.forM f := by induction t <;> simp [*]
 
+@[deprecated "Use `Std.TreeMap` instead." (since := "2026-05-05")]
 theorem foldlM_eq_foldlM_toList [Monad m] [LawfulMonad m] {t : RBNode α} :
     t.foldlM (m := m) f init = t.toList.foldlM f init := by
   induction t generalizing init <;> simp [*]
 
+@[deprecated "Use `Std.TreeMap` instead." (since := "2026-05-05")]
 theorem forIn_visit_eq_bindList [Monad m] [LawfulMonad m] {t : RBNode α} :
     forIn.visit (m := m) f t init = (ForInStep.yield init).bindList f t.toList := by
   induction t generalizing init <;> simp [*, forIn.visit]
 
+@[deprecated "Use `Std.TreeMap` instead." (since := "2026-05-05")]
 theorem forIn_eq_forIn_toList [Monad m] [LawfulMonad m] {t : RBNode α} :
     forIn (m := m) t init f = forIn t.toList init f := by
   conv => lhs; simp only [forIn, RBNode.forIn]
@@ -201,21 +239,27 @@ namespace Stream
 
 attribute [simp] foldl foldr
 
+@[deprecated "Use `Std.TreeMap` instead." (since := "2026-05-05")]
 theorem foldr_cons (t : RBNode.Stream α) (l) : t.foldr (·::·) l = t.toList ++ l := by
   unfold toList; apply Eq.symm; induction t <;> simp [*, foldr, RBNode.foldr_cons]
 
-@[simp] theorem toList_nil : (.nil : RBNode.Stream α).toList = [] := rfl
+@[deprecated "Use `Std.TreeMap` instead." (since := "2026-05-05"), simp]
+theorem toList_nil : (.nil : RBNode.Stream α).toList = [] := rfl
 
-@[simp] theorem toList_cons :
+@[deprecated "Use `Std.TreeMap` instead." (since := "2026-05-05"), simp]
+theorem toList_cons :
     (.cons x r s : RBNode.Stream α).toList = x :: r.toList ++ s.toList := by
   rw [toList, toList, foldr, RBNode.foldr_cons]; rfl
 
+@[deprecated "Use `Std.TreeMap` instead." (since := "2026-05-05")]
 theorem foldr_eq_foldr_toList {s : RBNode.Stream α} : s.foldr f init = s.toList.foldr f init := by
   induction s <;> simp [*, RBNode.foldr_eq_foldr_toList]
 
+@[deprecated "Use `Std.TreeMap` instead." (since := "2026-05-05")]
 theorem foldl_eq_foldl_toList {t : RBNode.Stream α} : t.foldl f init = t.toList.foldl f init := by
   induction t generalizing init <;> simp [*, RBNode.foldl_eq_foldl_toList]
 
+@[deprecated "Use `Std.TreeMap` instead." (since := "2026-05-05")]
 theorem forIn_eq_forIn_toList [Monad m] [LawfulMonad m] {t : RBNode α} :
     forIn (m := m) t init f = forIn t.toList init f := by
   conv => lhs; simp only [forIn, RBNode.forIn]
@@ -223,16 +267,20 @@ theorem forIn_eq_forIn_toList [Monad m] [LawfulMonad m] {t : RBNode α} :
 
 end Stream
 
+@[deprecated "Use `Std.TreeMap` instead." (since := "2026-05-05")]
 theorem toStream_toList' {t : RBNode α} {s} : (t.toStream s).toList = t.toList ++ s.toList := by
   induction t generalizing s <;> simp [*, toStream]
 
-@[simp] theorem toStream_toList {t : RBNode α} : t.toStream.toList = t.toList := by
+@[deprecated "Use `Std.TreeMap` instead." (since := "2026-05-05"), simp]
+theorem toStream_toList {t : RBNode α} : t.toStream.toList = t.toList := by
   simp [toStream_toList']
 
+@[deprecated "Use `Std.TreeMap` instead." (since := "2026-05-05")]
 theorem Stream.next?_toList {s : RBNode.Stream α} :
     (s.next?.map fun (a, b) => (a, b.toList)) = s.toList.next? := by
   cases s <;> simp [next?, toStream_toList']
 
+@[deprecated "Use `Std.TreeMap` instead." (since := "2026-05-05")]
 theorem ordered_iff {t : RBNode α} :
     t.Ordered cmp ↔ t.toList.Pairwise (cmpLT cmp) := by
   induction t with
@@ -242,14 +290,17 @@ theorem ordered_iff {t : RBNode α} :
       and_assoc, and_left_comm, and_comm, imp_and, forall_and]
     exact fun _ _ hl hr a ha b hb => (hl _ ha).trans (hr _ hb)
 
+@[deprecated "Use `Std.TreeMap` instead." (since := "2026-05-05")]
 theorem Ordered.toList_sorted {t : RBNode α} : t.Ordered cmp → t.toList.Pairwise (cmpLT cmp) :=
   ordered_iff.1
 
+@[deprecated "Use `Std.TreeMap` instead." (since := "2026-05-05")]
 theorem min?_mem {t : RBNode α} (h : t.min? = some a) : a ∈ t := by
   rw [min?_eq_toList_head?] at h
   rw [← mem_toList]
   revert h; cases toList t <;> rintro ⟨⟩; constructor
 
+@[deprecated "Use `Std.TreeMap` instead." (since := "2026-05-05")]
 theorem Ordered.min?_le {t : RBNode α} [Std.TransCmp cmp] (ht : t.Ordered cmp)
     (h : t.min? = some a) (x) (hx : x ∈ t) : cmp a x ≠ .gt := by
   rw [min?_eq_toList_head?] at h
@@ -259,61 +310,78 @@ theorem Ordered.min?_le {t : RBNode α} [Std.TransCmp cmp] (ht : t.Ordered cmp)
   · rw [Std.ReflCmp.compare_self (cmp := cmp)]; decide
   · rw [(h1 _ hx).1]; decide
 
+@[deprecated "Use `Std.TreeMap` instead." (since := "2026-05-05")]
 theorem max?_mem {t : RBNode α} (h : t.max? = some a) : a ∈ t := by
   simpa using min?_mem ((min?_reverse _).trans h)
 
+@[deprecated "Use `Std.TreeMap` instead." (since := "2026-05-05")]
 theorem Ordered.le_max? {t : RBNode α} [Std.TransCmp cmp] (ht : t.Ordered cmp)
     (h : t.max? = some a) (x) (hx : x ∈ t) : cmp x a ≠ .gt :=
   ht.reverse.min?_le ((min?_reverse _).trans h) _ (by simpa using hx)
 
-@[simp] theorem setBlack_toList {t : RBNode α} : t.setBlack.toList = t.toList := by
+@[deprecated "Use `Std.TreeMap` instead." (since := "2026-05-05"), simp]
+theorem setBlack_toList {t : RBNode α} : t.setBlack.toList = t.toList := by
   cases t <;> simp [setBlack]
 
-@[simp] theorem setRed_toList {t : RBNode α} : t.setRed.toList = t.toList := by
+@[deprecated "Use `Std.TreeMap` instead." (since := "2026-05-05"), simp]
+theorem setRed_toList {t : RBNode α} : t.setRed.toList = t.toList := by
   cases t <;> simp [setRed]
 
-@[simp] theorem balance1_toList {l : RBNode α} {v r} :
+@[deprecated "Use `Std.TreeMap` instead." (since := "2026-05-05"), simp]
+theorem balance1_toList {l : RBNode α} {v r} :
     (l.balance1 v r).toList = l.toList ++ v :: r.toList := by
   unfold balance1; split <;> simp
 
-@[simp] theorem balance2_toList {l : RBNode α} {v r} :
+@[deprecated "Use `Std.TreeMap` instead." (since := "2026-05-05"), simp]
+theorem balance2_toList {l : RBNode α} {v r} :
     (l.balance2 v r).toList = l.toList ++ v :: r.toList := by
   unfold balance2; split <;> simp
 
-@[simp] theorem balLeft_toList {l : RBNode α} {v r} :
+@[deprecated "Use `Std.TreeMap` instead." (since := "2026-05-05"), simp]
+theorem balLeft_toList {l : RBNode α} {v r} :
     (l.balLeft v r).toList = l.toList ++ v :: r.toList := by
   unfold balLeft; split <;> (try simp); split <;> simp
 
-@[simp] theorem balRight_toList {l : RBNode α} {v r} :
+@[deprecated "Use `Std.TreeMap` instead." (since := "2026-05-05"), simp]
+theorem balRight_toList {l : RBNode α} {v r} :
     (l.balRight v r).toList = l.toList ++ v :: r.toList := by
   unfold balRight; split <;> (try simp); split <;> simp
 
+@[deprecated "Use `Std.TreeMap` instead." (since := "2026-05-05")]
 theorem size_eq {t : RBNode α} : t.size = t.toList.length := by
   induction t <;> simp [*, size]; rfl
 
-@[simp] theorem reverse_size (t : RBNode α) : t.reverse.size = t.size := by simp [size_eq]
+@[deprecated "Use `Std.TreeMap` instead." (since := "2026-05-05"), simp]
+theorem reverse_size (t : RBNode α) : t.reverse.size = t.size := by simp [size_eq]
 
-@[simp] theorem Any_reverse {t : RBNode α} : t.reverse.Any p ↔ t.Any p := by simp [Any_def]
+@[deprecated "Use `Std.TreeMap` instead." (since := "2026-05-05"), simp]
+theorem Any_reverse {t : RBNode α} : t.reverse.Any p ↔ t.Any p := by simp [Any_def]
 
-@[simp] theorem memP_reverse {t : RBNode α} : MemP cut t.reverse ↔ MemP (cut · |>.swap) t := by
+@[deprecated "Use `Std.TreeMap` instead." (since := "2026-05-05"), simp]
+theorem memP_reverse {t : RBNode α} : MemP cut t.reverse ↔ MemP (cut · |>.swap) t := by
   simp [MemP]
 
+@[deprecated "Use `Std.TreeMap` instead." (since := "2026-05-05")]
 theorem Mem_reverse [Std.OrientedCmp (α := α) cmp] {t : RBNode α} :
     Mem cmp x t.reverse ↔ Mem (flip cmp) x t := by
   simp [Mem]; apply Iff.of_eq; congr; funext x; rw [← Std.OrientedCmp.eq_swap]; rfl
 
 section find?
 
+@[deprecated "Use `Std.TreeMap` instead." (since := "2026-05-05")]
 theorem find?_some_eq_eq {t : RBNode α} : x ∈ t.find? cut → cut x = .eq := by
   induction t <;> simp [find?]; split <;> try assumption
   intro | rfl => assumption
 
+@[deprecated "Use `Std.TreeMap` instead." (since := "2026-05-05")]
 theorem find?_some_mem {t : RBNode α} : x ∈ t.find? cut → x ∈ t := by
   induction t <;> simp [find?]; split <;> simp (config := {contextual := true}) [*]
 
+@[deprecated "Use `Std.TreeMap` instead." (since := "2026-05-05")]
 theorem find?_some_memP {t : RBNode α} (h : x ∈ t.find? cut) : MemP cut t :=
   memP_def.2 ⟨_, find?_some_mem h, find?_some_eq_eq h⟩
 
+@[deprecated "Use `Std.TreeMap` instead." (since := "2026-05-05")]
 theorem Ordered.memP_iff_find? [Std.TransCmp (α := α) cmp] [IsCut cmp cut]
     (ht : Ordered cmp t) : MemP cut t ↔ ∃ x, t.find? cut = some x := by
   refine ⟨fun H => ?_, fun ⟨x, h⟩ => find?_some_memP h⟩
@@ -338,6 +406,7 @@ theorem Ordered.memP_iff_find? [Std.TransCmp (α := α) cmp] [IsCut cmp cut]
       · exact hx
     · exact ⟨_, rfl⟩
 
+@[deprecated "Use `Std.TreeMap` instead." (since := "2026-05-05")]
 theorem Ordered.unique [Std.TransCmp (α := α) cmp] (ht : Ordered cmp t)
     (hx : x ∈ t) (hy : y ∈ t) (e : cmp x y = .eq) : x = y := by
   induction t with
@@ -356,13 +425,15 @@ theorem Ordered.unique [Std.TransCmp (α := α) cmp] (ht : Ordered cmp t)
         ((All_def.1 lx _ hy).trans (All_def.1 xr _ hx)).1
     · exact ihr hr hx hy
 
+@[deprecated "Use `Std.TreeMap` instead." (since := "2026-05-05")]
 theorem Ordered.find?_some [Std.TransCmp (α := α) cmp] [IsStrictCut cmp cut]
     (ht : Ordered cmp t) : t.find? cut = some x ↔ x ∈ t ∧ cut x = .eq := by
   refine ⟨fun h => ⟨find?_some_mem h, find?_some_eq_eq h⟩, fun ⟨hx, e⟩ => ?_⟩
   have ⟨y, hy⟩ := ht.memP_iff_find?.1 (memP_def.2 ⟨_, hx, e⟩)
   exact ht.unique hx (find?_some_mem hy) ((IsStrictCut.exact e).trans (find?_some_eq_eq hy)) ▸ hy
 
-@[simp] theorem find?_reverse (t : RBNode α) (cut : α → Ordering) :
+@[deprecated "Use `Std.TreeMap` instead." (since := "2026-05-05"), simp]
+theorem find?_reverse (t : RBNode α) (cut : α → Ordering) :
     t.reverse.find? cut = t.find? (cut · |>.swap) := by
   induction t <;> simp [*, find?]
   cases cut _ <;> simp [Ordering.swap]
@@ -370,6 +441,7 @@ theorem Ordered.find?_some [Std.TransCmp (α := α) cmp] [IsStrictCut cmp cut]
 /--
 Auxiliary definition for `zoom_ins`: set the root of the tree to `v`, creating a node if necessary.
 -/
+@[deprecated "Use `Std.TreeMap` instead." (since := "2026-05-05")]
 def setRoot (v : α) : RBNode α → RBNode α
   | nil => node red nil v nil
   | node c a _ b => node c a v b
@@ -377,6 +449,7 @@ def setRoot (v : α) : RBNode α → RBNode α
 /--
 Auxiliary definition for `zoom_ins`: set the root of the tree to `v`, creating a node if necessary.
 -/
+@[deprecated "Use `Std.TreeMap` instead." (since := "2026-05-05")]
 def delRoot : RBNode α → RBNode α
   | nil => nil
   | node _ a _ b => a.append b
@@ -385,15 +458,18 @@ end find?
 
 section «upperBound? and lowerBound?»
 
-@[simp] theorem upperBound?_reverse (t : RBNode α) (cut ub) :
+@[deprecated "Use `Std.TreeMap` instead." (since := "2026-05-05"), simp]
+theorem upperBound?_reverse (t : RBNode α) (cut ub) :
     t.reverse.upperBound? cut ub = t.lowerBound? (cut · |>.swap) ub := by
   induction t generalizing ub <;> simp [lowerBound?, upperBound?]
   split <;> simp [*, Ordering.swap]
 
-@[simp] theorem lowerBound?_reverse (t : RBNode α) (cut lb) :
+@[deprecated "Use `Std.TreeMap` instead." (since := "2026-05-05"), simp]
+theorem lowerBound?_reverse (t : RBNode α) (cut lb) :
     t.reverse.lowerBound? cut lb = t.upperBound? (cut · |>.swap) lb := by
   simpa using (upperBound?_reverse t.reverse (cut · |>.swap) lb).symm
 
+@[deprecated "Use `Std.TreeMap` instead." (since := "2026-05-05")]
 theorem upperBound?_eq_find? {t : RBNode α} {cut} (ub) (H : t.find? cut = some x) :
     t.upperBound? cut ub = some x := by
   induction t generalizing ub with simp [find?] at H
@@ -403,12 +479,14 @@ theorem upperBound?_eq_find? {t : RBNode α} {cut} (ub) (H : t.find? cut = some 
     · apply ihb _ H
     · exact H
 
+@[deprecated "Use `Std.TreeMap` instead." (since := "2026-05-05")]
 theorem lowerBound?_eq_find? {t : RBNode α} {cut} (lb) (H : t.find? cut = some x) :
     t.lowerBound? cut lb = some x := by
   rw [← reverse_reverse t] at H ⊢; rw [lowerBound?_reverse]; rw [find?_reverse] at H
   exact upperBound?_eq_find? _ H
 
 /-- The value `x` returned by `upperBound?` is greater or equal to the `cut`. -/
+@[deprecated "Use `Std.TreeMap` instead." (since := "2026-05-05")]
 theorem upperBound?_ge' {t : RBNode α} (H : ∀ {x}, x ∈ ub → cut x ≠ .gt) :
     t.upperBound? cut ub = some x → cut x ≠ .gt := by
   induction t generalizing ub with
@@ -420,19 +498,23 @@ theorem upperBound?_ge' {t : RBNode α} (H : ∀ {x}, x ∈ ub → cut x ≠ .gt
     · next hv => intro | rfl, e => cases hv.symm.trans e
 
 /-- The value `x` returned by `upperBound?` is greater or equal to the `cut`. -/
+@[deprecated "Use `Std.TreeMap` instead." (since := "2026-05-05")]
 theorem upperBound?_ge {t : RBNode α} : t.upperBound? cut = some x → cut x ≠ .gt :=
   upperBound?_ge' nofun
 
 /-- The value `x` returned by `lowerBound?` is less or equal to the `cut`. -/
+@[deprecated "Use `Std.TreeMap` instead." (since := "2026-05-05")]
 theorem lowerBound?_le' {t : RBNode α} (H : ∀ {x}, x ∈ lb → cut x ≠ .lt) :
     t.lowerBound? cut lb = some x → cut x ≠ .lt := by
   rw [← reverse_reverse t, lowerBound?_reverse, Ne, ← Ordering.swap_inj]
   exact upperBound?_ge' fun h => by specialize H h; rwa [Ne, ← Ordering.swap_inj] at H
 
 /-- The value `x` returned by `lowerBound?` is less or equal to the `cut`. -/
+@[deprecated "Use `Std.TreeMap` instead." (since := "2026-05-05")]
 theorem lowerBound?_le {t : RBNode α} : t.lowerBound? cut = some x → cut x ≠ .lt :=
   lowerBound?_le' nofun
 
+@[deprecated "Use `Std.TreeMap` instead." (since := "2026-05-05")]
 theorem All.upperBound?_ub {t : RBNode α} (hp : t.All p) (H : ∀ {x}, ub = some x → p x) :
     t.upperBound? cut ub = some x → p x := by
   induction t generalizing ub with
@@ -443,37 +525,47 @@ theorem All.upperBound?_ub {t : RBNode α} (hp : t.All p) (H : ∀ {x}, ub = som
     · exact ihr hp.2.2 H
     · exact fun | rfl => hp.1
 
+@[deprecated "Use `Std.TreeMap` instead." (since := "2026-05-05")]
 theorem All.upperBound? {t : RBNode α} (hp : t.All p) : t.upperBound? cut = some x → p x :=
   hp.upperBound?_ub nofun
 
+@[deprecated "Use `Std.TreeMap` instead." (since := "2026-05-05")]
 theorem All.lowerBound?_lb {t : RBNode α} (hp : t.All p) (H : ∀ {x}, lb = some x → p x) :
     t.lowerBound? cut lb = some x → p x := by
   rw [← reverse_reverse t, lowerBound?_reverse]
   exact All.upperBound?_ub (All.reverse.2 hp) H
 
+@[deprecated "Use `Std.TreeMap` instead." (since := "2026-05-05")]
 theorem All.lowerBound? {t : RBNode α} (hp : t.All p) : t.lowerBound? cut = some x → p x :=
   hp.lowerBound?_lb nofun
 
+@[deprecated "Use `Std.TreeMap` instead." (since := "2026-05-05")]
 theorem upperBound?_mem_ub {t : RBNode α}
     (h : t.upperBound? cut ub = some x) : x ∈ t ∨ ub = some x :=
   All.upperBound?_ub (p := fun x => x ∈ t ∨ ub = some x) (All_def.2 fun _ => .inl) Or.inr h
 
+@[deprecated "Use `Std.TreeMap` instead." (since := "2026-05-05")]
 theorem upperBound?_mem {t : RBNode α} (h : t.upperBound? cut = some x) : x ∈ t :=
   (upperBound?_mem_ub h).resolve_right nofun
 
+@[deprecated "Use `Std.TreeMap` instead." (since := "2026-05-05")]
 theorem lowerBound?_mem_lb {t : RBNode α}
     (h : t.lowerBound? cut lb = some x) : x ∈ t ∨ lb = some x :=
   All.lowerBound?_lb (p := fun x => x ∈ t ∨ lb = some x) (All_def.2 fun _ => .inl) Or.inr h
 
+@[deprecated "Use `Std.TreeMap` instead." (since := "2026-05-05")]
 theorem lowerBound?_mem {t : RBNode α} (h : t.lowerBound? cut = some x) : x ∈ t :=
   (lowerBound?_mem_lb h).resolve_right nofun
 
+@[deprecated "Use `Std.TreeMap` instead." (since := "2026-05-05")]
 theorem upperBound?_of_some {t : RBNode α} : ∃ x, t.upperBound? cut (some y) = some x := by
   induction t generalizing y <;> simp [upperBound?]; split <;> simp [*]
 
+@[deprecated "Use `Std.TreeMap` instead." (since := "2026-05-05")]
 theorem lowerBound?_of_some {t : RBNode α} : ∃ x, t.lowerBound? cut (some y) = some x := by
   rw [← reverse_reverse t, lowerBound?_reverse]; exact upperBound?_of_some
 
+@[deprecated "Use `Std.TreeMap` instead." (since := "2026-05-05")]
 theorem Ordered.upperBound?_exists [Std.TransCmp (α := α) cmp] [IsCut cmp cut]
     (h : Ordered cmp t) : (∃ x, t.upperBound? cut = some x) ↔ ∃ x ∈ t, cut x ≠ .gt := by
   refine ⟨fun ⟨x, hx⟩ => ⟨_, upperBound?_mem hx, upperBound?_ge hx⟩, fun H => ?_⟩
@@ -489,12 +581,14 @@ theorem Ordered.upperBound?_exists [Std.TransCmp (α := α) cmp] [IsCut cmp cut]
       · exact ihr h.2.2.2 _ hx e
     · exact ⟨_, rfl⟩
 
+@[deprecated "Use `Std.TreeMap` instead." (since := "2026-05-05")]
 theorem Ordered.lowerBound?_exists [Std.TransCmp (α := α) cmp] [IsCut cmp cut]
     (h : Ordered cmp t) : (∃ x, t.lowerBound? cut = some x) ↔ ∃ x ∈ t, cut x ≠ .lt := by
   conv => enter [2, 1, x]; rw [Ne, ← Ordering.swap_inj]
   rw [← reverse_reverse t, lowerBound?_reverse]
   simpa [-Ordering.swap_inj] using h.reverse.upperBound?_exists (cut := (cut · |>.swap))
 
+@[deprecated "Use `Std.TreeMap` instead." (since := "2026-05-05")]
 theorem Ordered.upperBound?_least_ub [Std.TransCmp (α := α) cmp] [IsCut cmp cut]
     (h : Ordered cmp t) (hub : ∀ {x}, ub = some x → t.All (cmpLT cmp · x)) :
     t.upperBound? cut ub = some x → y ∈ t → cut x = .lt → cmp y x = .lt → cut y = .gt := by
@@ -517,6 +611,7 @@ theorem Ordered.upperBound?_least_ub [Std.TransCmp (α := α) cmp] [IsCut cmp cu
     · cases h₁; cases hx.symm.trans hv
     · cases h₁; cases hx.symm.trans hv
 
+@[deprecated "Use `Std.TreeMap` instead." (since := "2026-05-05")]
 theorem Ordered.lowerBound?_greatest_lb [Std.TransCmp (α := α) cmp] [IsCut cmp cut]
     (h : Ordered cmp t) (hlb : ∀ {x}, lb = some x → t.All (cmpLT cmp x ·)) :
     t.lowerBound? cut lb = some x → y ∈ t → cut x = .gt → cmp x y = .lt → cut y = .lt := by
@@ -532,6 +627,7 @@ A statement of the least-ness of the result of `upperBound?`. If `x` is the retu
 `upperBound?` and it is strictly greater than the cut, then any other `y < x` in the tree is in fact
 strictly less than the cut (so there is no exact match, and nothing closer to the cut).
 -/
+@[deprecated "Use `Std.TreeMap` instead." (since := "2026-05-05")]
 theorem Ordered.upperBound?_least [Std.TransCmp (α := α) cmp] [IsCut cmp cut]
     (ht : Ordered cmp t) (H : t.upperBound? cut = some x) (hy : y ∈ t)
     (xy : cmp y x = .lt) (hx : cut x = .lt) : cut y = .gt :=
@@ -542,11 +638,13 @@ A statement of the greatest-ness of the result of `lowerBound?`. If `x` is the r
 `lowerBound?` and it is strictly less than the cut, then any other `y > x` in the tree is in fact
 strictly greater than the cut (so there is no exact match, and nothing closer to the cut).
 -/
+@[deprecated "Use `Std.TreeMap` instead." (since := "2026-05-05")]
 theorem Ordered.lowerBound?_greatest [Std.TransCmp (α := α) cmp] [IsCut cmp cut]
     (ht : Ordered cmp t) (H : t.lowerBound? cut none = some x) (hy : y ∈ t)
     (xy : cmp x y = .lt) (hx : cut x = .gt) : cut y = .lt :=
   ht.lowerBound?_greatest_lb (by nofun) H hy hx xy
 
+@[deprecated "Use `Std.TreeMap` instead." (since := "2026-05-05")]
 theorem Ordered.memP_iff_upperBound? [Std.TransCmp (α := α) cmp] [IsCut cmp cut]
     (ht : Ordered cmp t) : t.MemP cut ↔ ∃ x, t.upperBound? cut = some x ∧ cut x = .eq := by
   refine memP_def.trans ⟨fun ⟨y, hy, ey⟩ => ?_, fun ⟨x, hx, e⟩ => ⟨_, upperBound?_mem hx, e⟩⟩
@@ -559,6 +657,7 @@ theorem Ordered.memP_iff_upperBound? [Std.TransCmp (α := α) cmp] [IsCut cmp cu
   · rfl
   · cases upperBound?_ge hx ex
 
+@[deprecated "Use `Std.TreeMap` instead." (since := "2026-05-05")]
 theorem Ordered.memP_iff_lowerBound? [Std.TransCmp (α := α) cmp] [IsCut cmp cut]
     (ht : Ordered cmp t) : t.MemP cut ↔ ∃ x, t.lowerBound? cut = some x ∧ cut x = .eq := by
   refine memP_def.trans ⟨fun ⟨y, hy, ey⟩ => ?_, fun ⟨x, hx, e⟩ => ⟨_, lowerBound?_mem hx, e⟩⟩
@@ -572,6 +671,7 @@ theorem Ordered.memP_iff_lowerBound? [Std.TransCmp (α := α) cmp] [IsCut cmp cu
     · cases ey.symm.trans <| IsCut.gt_trans (Std.OrientedCmp.gt_iff_lt.1 e) ex
 
 /-- A stronger version of `lowerBound?_greatest` that holds when the cut is strict. -/
+@[deprecated "Use `Std.TreeMap` instead." (since := "2026-05-05")]
 theorem Ordered.lowerBound?_lt [Std.TransCmp (α := α) cmp] [IsStrictCut cmp cut]
     (ht : Ordered cmp t) (H : t.lowerBound? cut = some x) (hy : y ∈ t) :
     cmp x y = .lt ↔ cut y = .lt := by
@@ -583,6 +683,7 @@ theorem Ordered.lowerBound?_lt [Std.TransCmp (α := α) cmp] [IsStrictCut cmp cu
   · by_contra h'; exact lowerBound?_le H <| IsCut.le_lt_trans (cmp := cmp) (cut := cut) h' h
 
 /-- A stronger version of `upperBound?_least` that holds when the cut is strict. -/
+@[deprecated "Use `Std.TreeMap` instead." (since := "2026-05-05")]
 theorem Ordered.lt_upperBound? [Std.TransCmp (α := α) cmp] [IsStrictCut cmp cut]
     (ht : Ordered cmp t) (H : t.upperBound? cut = some x) (hy : y ∈ t) :
     cmp y x = .lt ↔ cut y = .gt := by
@@ -598,21 +699,25 @@ attribute [simp] RootOrdered Ordered
 
 /-- The list of elements to the left of the hole.
 (This function is intended for specification purposes only.) -/
-@[simp] def listL : Path α → List α
+@[deprecated "Use `Std.TreeMap` instead." (since := "2026-05-05"), simp]
+def listL : Path α → List α
   | .root => []
   | .left _ parent _ _ => parent.listL
   | .right _ l v parent => parent.listL ++ (l.toList ++ [v])
 
 /-- The list of elements to the right of the hole.
 (This function is intended for specification purposes only.) -/
-@[simp] def listR : Path α → List α
+@[deprecated "Use `Std.TreeMap` instead." (since := "2026-05-05"), simp]
+def listR : Path α → List α
   | .root => []
   | .left _ parent v r => v :: r.toList ++ parent.listR
   | .right _ _ _ parent => parent.listR
 
 /-- Wraps a list of elements with the left and right elements of the path. -/
+@[deprecated "Use `Std.TreeMap` instead." (since := "2026-05-05")]
 abbrev withList (p : Path α) (l : List α) : List α := p.listL ++ l ++ p.listR
 
+@[deprecated "Use `Std.TreeMap` instead." (since := "2026-05-05")]
 theorem rootOrdered_iff {p : Path α} (hp : p.Ordered cmp) :
     p.RootOrdered cmp v ↔ (∀ a ∈ p.listL, cmpLT cmp a v) ∧ (∀ a ∈ p.listR, cmpLT cmp v a) := by
   induction p with
@@ -620,6 +725,7 @@ theorem rootOrdered_iff {p : Path α} (hp : p.Ordered cmp) :
   | left _ _ x _ ih => exact fun vx _ _ _ ha => vx.trans (hp.2.1 _ ha)
   | right _ _ x _ ih => exact fun xv _ _ _ ha => (hp.2.1 _ ha).trans xv
 
+@[deprecated "Use `Std.TreeMap` instead." (since := "2026-05-05")]
 theorem ordered_iff {p : Path α} :
     p.Ordered cmp ↔ p.listL.Pairwise (cmpLT cmp) ∧ p.listR.Pairwise (cmpLT cmp) ∧
       ∀ x ∈ p.listL, ∀ y ∈ p.listR, cmpLT cmp x y := by
@@ -641,6 +747,7 @@ theorem ordered_iff {p : Path α} :
       fun ⟨⟨hL, ⟨hl, lx⟩, Ll, Lx⟩, hR, LR, lR, xR⟩ =>
        ⟨⟨hL, hR, LR⟩, lx, ⟨Lx, xR⟩, ⟨fun _ ha _ hb => Ll _ hb _ ha, lR⟩, hl⟩⟩
 
+@[deprecated "Use `Std.TreeMap` instead." (since := "2026-05-05")]
 theorem zoom_zoomed₁ (e : zoom cut t path = (t', path')) :
     t'.OnRoot (cut · = .eq) :=
   match t, e with
@@ -651,30 +758,37 @@ theorem zoom_zoomed₁ (e : zoom cut t path = (t', path')) :
     · exact zoom_zoomed₁
     · next H => intro e; cases e; exact H
 
-@[simp] theorem fill_toList {p : Path α} : (p.fill t).toList = p.withList t.toList := by
+@[deprecated "Use `Std.TreeMap` instead." (since := "2026-05-05"), simp]
+theorem fill_toList {p : Path α} : (p.fill t).toList = p.withList t.toList := by
   induction p generalizing t <;> simp [*]
 
+@[deprecated "Use `Std.TreeMap` instead." (since := "2026-05-05")]
 theorem _root_.Batteries.RBNode.zoom_toList {t : RBNode α} (eq : t.zoom cut = (t', p')) :
     p'.withList t'.toList = t.toList := by rw [← fill_toList, ← zoom_fill eq]; rfl
 
-@[simp] theorem ins_toList {p : Path α} : (p.ins t).toList = p.withList t.toList := by
+@[deprecated "Use `Std.TreeMap` instead." (since := "2026-05-05"), simp]
+theorem ins_toList {p : Path α} : (p.ins t).toList = p.withList t.toList := by
   match p with
   | .root | .left red .. | .right red .. | .left black .. | .right black .. =>
     simp [ins, ins_toList]
 
-@[simp] theorem insertNew_toList {p : Path α} : (p.insertNew v).toList = p.withList [v] := by
+@[deprecated "Use `Std.TreeMap` instead." (since := "2026-05-05"), simp]
+theorem insertNew_toList {p : Path α} : (p.insertNew v).toList = p.withList [v] := by
   simp [insertNew]
 
+@[deprecated "Use `Std.TreeMap` instead." (since := "2026-05-05")]
 theorem insert_toList {p : Path α} :
     (p.insert t v).toList = p.withList (t.setRoot v).toList := by
   simp [insert]; split <;> simp [setRoot]
 
+@[deprecated "Use `Std.TreeMap` instead." (since := "2026-05-05")]
 protected theorem Balanced.insert {path : Path α} (hp : path.Balanced c₀ n₀ c n) :
     t.Balanced c n → ∃ c n, (path.insert t v).Balanced c n
   | .nil => ⟨_, hp.insertNew⟩
   | .red ha hb => ⟨_, _, hp.fill (.red ha hb)⟩
   | .black ha hb => ⟨_, _, hp.fill (.black ha hb)⟩
 
+@[deprecated "Use `Std.TreeMap` instead." (since := "2026-05-05")]
 theorem Ordered.insert : ∀ {path : Path α} {t : RBNode α},
     path.Ordered cmp → t.Ordered cmp → t.All (path.RootOrdered cmp) → path.RootOrdered cmp v →
     t.OnRoot (cmpEq cmp v) → (path.insert t v).Ordered cmp
@@ -682,11 +796,13 @@ theorem Ordered.insert : ∀ {path : Path α} {t : RBNode α},
   | _, node .., hp, ⟨ax, xb, ha, hb⟩, ⟨_, ap, bp⟩, vp, xv => Ordered.fill.2
     ⟨hp, ⟨ax.imp xv.lt_congr_right.2, xb.imp xv.lt_congr_left.2, ha, hb⟩, vp, ap, bp⟩
 
+@[deprecated "Use `Std.TreeMap` instead." (since := "2026-05-05")]
 theorem Ordered.erase : ∀ {path : Path α} {t : RBNode α},
     path.Ordered cmp → t.Ordered cmp → t.All (path.RootOrdered cmp) → (path.erase t).Ordered cmp
   | _, nil, hp, ht, tp => Ordered.fill.2 ⟨hp, ht, tp⟩
   | _, node .., hp, ⟨ax, xb, ha, hb⟩, ⟨_, ap, bp⟩ => hp.del (ha.append ax xb hb) (ap.append bp)
 
+@[deprecated "Use `Std.TreeMap` instead." (since := "2026-05-05")]
 theorem zoom_ins {t : RBNode α} {cmp : α → α → Ordering} :
     t.zoom (cmp v) path = (t', path') →
     path.ins (t.ins cmp v) = path'.ins (t'.setRoot v) := by
@@ -698,10 +814,12 @@ theorem zoom_ins {t : RBNode α} {cmp : α → α → Ordering} :
     · exact zoom_ins
     · intro | rfl => rfl
 
+@[deprecated "Use `Std.TreeMap` instead." (since := "2026-05-05")]
 theorem insertNew_eq_insert (h : zoom (cmp v) t = (nil, path)) :
     path.insertNew v = (t.insert cmp v).setBlack :=
   insert_setBlack .. ▸ (zoom_ins h).symm
 
+@[deprecated "Use `Std.TreeMap` instead." (since := "2026-05-05")]
 theorem ins_eq_fill {path : Path α} {t : RBNode α} :
     path.Balanced c₀ n₀ c n → t.Balanced c n → path.ins t = (path.fill t).setBlack
   | .root, h => rfl
@@ -709,6 +827,7 @@ theorem ins_eq_fill {path : Path α} {t : RBNode α} :
   | .blackL hb H, ha => by rw [ins, fill, ← ins_eq_fill H (.black ha hb), balance1_eq ha]
   | .blackR ha H, hb => by rw [ins, fill, ← ins_eq_fill H (.black ha hb), balance2_eq hb]
 
+@[deprecated "Use `Std.TreeMap` instead." (since := "2026-05-05")]
 theorem zoom_insert {path : Path α} {t : RBNode α} (ht : t.Balanced c n)
     (H : zoom (cmp v) t = (t', path)) :
     (path.insert t' v).setBlack = (t.insert cmp v).setBlack := by
@@ -718,6 +837,7 @@ theorem zoom_insert {path : Path α} {t : RBNode α} (ht : t.Balanced c n)
   | red hl hr => rw [← ins_eq_fill hp' (.red hl hr), insert_setBlack]; exact (zoom_ins H).symm
   | black hl hr => rw [← ins_eq_fill hp' (.black hl hr), insert_setBlack]; exact (zoom_ins H).symm
 
+@[deprecated "Use `Std.TreeMap` instead." (since := "2026-05-05")]
 theorem zoom_del {t : RBNode α} :
     t.zoom cut path = (t', path') →
     path.del (t.del cut) (match t with | node c .. => c | _ => red) =
@@ -737,12 +857,14 @@ theorem zoom_del {t : RBNode α} :
     · intro | rfl => rfl
 
 /-- Asserts that `p` holds on all elements to the left of the hole. -/
+@[deprecated "Use `Std.TreeMap` instead." (since := "2026-05-05")]
 def AllL (p : α → Prop) : Path α → Prop
   | .root => True
   | .left _ parent _ _ => parent.AllL p
   | .right _ a x parent => a.All p ∧ p x ∧ parent.AllL p
 
 /-- Asserts that `p` holds on all elements to the right of the hole. -/
+@[deprecated "Use `Std.TreeMap` instead." (since := "2026-05-05")]
 def AllR (p : α → Prop) : Path α → Prop
   | .root => True
   | .left _ parent x b => parent.AllR p ∧ p x ∧ b.All p
@@ -750,36 +872,43 @@ def AllR (p : α → Prop) : Path α → Prop
 
 end Path
 
+@[deprecated "Use `Std.TreeMap` instead." (since := "2026-05-05")]
 theorem insert_toList_zoom {t : RBNode α} (ht : Balanced t c n)
     (e : zoom (cmp v) t = (t', p)) :
     (t.insert cmp v).toList = p.withList (t'.setRoot v).toList := by
   rw [← setBlack_toList, ← Path.zoom_insert ht e, setBlack_toList, Path.insert_toList]
 
+@[deprecated "Use `Std.TreeMap` instead." (since := "2026-05-05")]
 theorem insert_toList_zoom_nil {t : RBNode α} (ht : Balanced t c n)
     (e : zoom (cmp v) t = (nil, p)) :
     (t.insert cmp v).toList = p.withList [v] := insert_toList_zoom ht e
 
+@[deprecated "Use `Std.TreeMap` instead." (since := "2026-05-05")]
 theorem exists_insert_toList_zoom_nil {t : RBNode α} (ht : Balanced t c n)
     (e : zoom (cmp v) t = (nil, p)) :
     ∃ L R, t.toList = L ++ R ∧ (t.insert cmp v).toList = L ++ v :: R :=
   ⟨p.listL, p.listR, by simp [← zoom_toList e, insert_toList_zoom_nil ht e]⟩
 
+@[deprecated "Use `Std.TreeMap` instead." (since := "2026-05-05")]
 theorem insert_toList_zoom_node {t : RBNode α} (ht : Balanced t c n)
     (e : zoom (cmp v) t = (node c' l v' r, p)) :
     (t.insert cmp v).toList = p.withList (node c l v r).toList := insert_toList_zoom ht e
 
+@[deprecated "Use `Std.TreeMap` instead." (since := "2026-05-05")]
 theorem exists_insert_toList_zoom_node {t : RBNode α} (ht : Balanced t c n)
     (e : zoom (cmp v) t = (node c' l v' r, p)) :
     ∃ L R, t.toList = L ++ v' :: R ∧ (t.insert cmp v).toList = L ++ v :: R := by
   refine ⟨p.listL ++ l.toList, r.toList ++ p.listR, ?_⟩
   simp [← zoom_toList e, insert_toList_zoom_node ht e]
 
+@[deprecated "Use `Std.TreeMap` instead." (since := "2026-05-05")]
 theorem mem_insert_self {t : RBNode α} (ht : Balanced t c n) : v ∈ t.insert cmp v := by
   rw [← mem_toList, List.mem_iff_append]
   exact match e : zoom (cmp v) t with
   | (nil, p) => let ⟨_, _, _, h⟩ := exists_insert_toList_zoom_nil ht e; ⟨_, _, h⟩
   | (node .., p) => let ⟨_, _, _, h⟩ := exists_insert_toList_zoom_node ht e; ⟨_, _, h⟩
 
+@[deprecated "Use `Std.TreeMap` instead." (since := "2026-05-05")]
 theorem mem_insert_of_mem {t : RBNode α} (ht : Balanced t c n) (h : v' ∈ t) :
     v' ∈ t.insert cmp v ∨ cmp v v' = .eq := by
   match e : zoom (cmp v) t with
@@ -793,16 +922,19 @@ theorem mem_insert_of_mem {t : RBNode α} (ht : Balanced t c n) (h : v' ∈ t) :
     simp [← mem_toList, h₂]; rcases h with h|h|h <;> simp [*]
     exact .inr (Path.zoom_zoomed₁ e)
 
+@[deprecated "Use `Std.TreeMap` instead." (since := "2026-05-05")]
 theorem exists_find?_insert_self [Std.TransCmp (α := α) cmp] [IsCut cmp cut]
     {t : RBNode α} (ht : Balanced t c n) (ht₂ : Ordered cmp t) (hv : cut v = .eq) :
     ∃ x, (t.insert cmp v).find? cut = some x :=
   ht₂.insert.memP_iff_find?.1 <| memP_def.2 ⟨_, mem_insert_self ht, hv⟩
 
+@[deprecated "Use `Std.TreeMap` instead." (since := "2026-05-05")]
 theorem find?_insert_self [Std.TransCmp (α := α) cmp] [IsStrictCut cmp cut]
     {t : RBNode α} (ht : Balanced t c n) (ht₂ : Ordered cmp t) (hv : cut v = .eq) :
     (t.insert cmp v).find? cut = some v :=
   ht₂.insert.find?_some.2 ⟨mem_insert_self ht, hv⟩
 
+@[deprecated "Use `Std.TreeMap` instead." (since := "2026-05-05")]
 theorem mem_insert [Std.TransCmp (α := α) cmp] {t : RBNode α}
     (ht : Balanced t c n) (ht₂ : Ordered cmp t) :
     v' ∈ t.insert cmp v ↔ (v' ∈ t ∧ t.find? (cmp v) ≠ some v') ∨ v' = v := by
@@ -832,124 +964,165 @@ open RBNode (IsCut IsStrictCut)
 
 namespace RBSet
 
-@[simp] theorem val_toList {t : RBSet α cmp} : t.1.toList = t.toList := rfl
+@[deprecated "Use `Std.TreeMap` instead." (since := "2026-05-05"), simp]
+theorem val_toList {t : RBSet α cmp} : t.1.toList = t.toList := rfl
 
-@[simp] theorem mkRBSet_eq : mkRBSet α cmp = ∅ := rfl
-@[simp] theorem empty_eq : @RBSet.empty α cmp = ∅ := rfl
-@[simp] theorem default_eq : (default : RBSet α cmp) = ∅ := rfl
-@[simp] theorem empty_toList : toList (∅ : RBSet α cmp) = [] := rfl
-@[simp] theorem single_toList : toList (single a : RBSet α cmp) = [a] := rfl
+@[deprecated "Use `Std.TreeMap` instead." (since := "2026-05-05"), simp]
+theorem mkRBSet_eq : mkRBSet α cmp = ∅ := rfl
+@[deprecated "Use `Std.TreeMap` instead." (since := "2026-05-05"), simp]
+theorem empty_eq : @RBSet.empty α cmp = ∅ := rfl
+@[deprecated "Use `Std.TreeMap` instead." (since := "2026-05-05"), simp]
+theorem default_eq : (default : RBSet α cmp) = ∅ := rfl
+@[deprecated "Use `Std.TreeMap` instead." (since := "2026-05-05"), simp]
+theorem empty_toList : toList (∅ : RBSet α cmp) = [] := rfl
+@[deprecated "Use `Std.TreeMap` instead." (since := "2026-05-05"), simp]
+theorem single_toList : toList (single a : RBSet α cmp) = [a] := rfl
 
+@[deprecated "Use `Std.TreeMap` instead." (since := "2026-05-05")]
 theorem mem_toList {t : RBSet α cmp} : x ∈ toList t ↔ x ∈ t.1 := RBNode.mem_toList
 
+@[deprecated "Use `Std.TreeMap` instead." (since := "2026-05-05")]
 theorem mem_congr [Std.TransCmp (α := α) cmp] {t : RBSet α cmp} (h : cmp x y = .eq) :
     x ∈ t ↔ y ∈ t := RBNode.mem_congr h
 
+@[deprecated "Use `Std.TreeMap` instead." (since := "2026-05-05")]
 theorem mem_iff_mem_toList {t : RBSet α cmp} : x ∈ t ↔ ∃ y ∈ toList t, cmp x y = .eq :=
   RBNode.mem_def.trans <| by simp [mem_toList]
 
+@[deprecated "Use `Std.TreeMap` instead." (since := "2026-05-05")]
 theorem mem_of_mem_toList [Std.OrientedCmp (α := α) cmp] {t : RBSet α cmp} (h : x ∈ toList t) :
     x ∈ t := mem_iff_mem_toList.2 ⟨_, h, Std.ReflCmp.compare_self⟩
 
+@[deprecated "Use `Std.TreeMap` instead." (since := "2026-05-05")]
 theorem foldl_eq_foldl_toList {t : RBSet α cmp} : t.foldl f init = t.toList.foldl f init :=
   RBNode.foldl_eq_foldl_toList
 
+@[deprecated "Use `Std.TreeMap` instead." (since := "2026-05-05")]
 theorem foldr_eq_foldr_toList {t : RBSet α cmp} : t.foldr f init = t.toList.foldr f init :=
   RBNode.foldr_eq_foldr_toList
 
+@[deprecated "Use `Std.TreeMap` instead." (since := "2026-05-05")]
 theorem foldlM_eq_foldlM_toList [Monad m] [LawfulMonad m] {t : RBSet α cmp} :
     t.foldlM (m := m) f init = t.toList.foldlM f init := RBNode.foldlM_eq_foldlM_toList
 
+@[deprecated "Use `Std.TreeMap` instead." (since := "2026-05-05")]
 theorem forM_eq_forM_toList [Monad m] [LawfulMonad m] {t : RBSet α cmp} :
     t.forM (m := m) f = t.toList.forM f := RBNode.forM_eq_forM_toList
 
+@[deprecated "Use `Std.TreeMap` instead." (since := "2026-05-05")]
 theorem forIn_eq_forIn_toList [Monad m] [LawfulMonad m] {t : RBSet α cmp} :
     forIn (m := m) t init f = forIn t.toList init f := RBNode.forIn_eq_forIn_toList
 
+@[deprecated "Use `Std.TreeMap` instead." (since := "2026-05-05")]
 theorem toStream_eq {t : RBSet α cmp} : Std.toStream t = t.1.toStream .nil := rfl
 
-@[simp] theorem toStream_toList {t : RBSet α cmp} : (Std.toStream t).toList = t.toList := by
+@[deprecated "Use `Std.TreeMap` instead." (since := "2026-05-05"), simp]
+theorem toStream_toList {t : RBSet α cmp} : (Std.toStream t).toList = t.toList := by
   simp [toStream_eq]
 
+@[deprecated "Use `Std.TreeMap` instead." (since := "2026-05-05")]
 theorem isEmpty_iff_toList_eq_nil {t : RBSet α cmp} :
     t.isEmpty ↔ t.toList = [] := by obtain ⟨⟨⟩, _⟩ := t <;> simp [toList, isEmpty]
 
+@[deprecated "Use `Std.TreeMap` instead." (since := "2026-05-05")]
 theorem toList_sorted {t : RBSet α cmp} : t.toList.Pairwise (RBNode.cmpLT cmp) :=
   t.2.out.1.toList_sorted
 
+@[deprecated "Use `Std.TreeMap` instead." (since := "2026-05-05")]
 theorem findP?_some_eq_eq {t : RBSet α cmp} : t.findP? cut = some y → cut y = .eq :=
   RBNode.find?_some_eq_eq
 
+@[deprecated "Use `Std.TreeMap` instead." (since := "2026-05-05")]
 theorem find?_some_eq_eq {t : RBSet α cmp} : t.find? x = some y → cmp x y = .eq :=
   findP?_some_eq_eq
 
+@[deprecated "Use `Std.TreeMap` instead." (since := "2026-05-05")]
 theorem findP?_some_mem_toList {t : RBSet α cmp} (h : t.findP? cut = some y) :
     y ∈ toList t := mem_toList.2 <| RBNode.find?_some_mem h
 
+@[deprecated "Use `Std.TreeMap` instead." (since := "2026-05-05")]
 theorem find?_some_mem_toList {t : RBSet α cmp} (h : t.find? x = some y) : y ∈ toList t :=
   findP?_some_mem_toList h
 
+@[deprecated "Use `Std.TreeMap` instead." (since := "2026-05-05")]
 theorem findP?_some_memP {t : RBSet α cmp} (h : t.findP? cut = some y) : t.MemP cut :=
   RBNode.find?_some_memP h
 
+@[deprecated "Use `Std.TreeMap` instead." (since := "2026-05-05")]
 theorem find?_some_mem {t : RBSet α cmp} (h : t.find? x = some y) : x ∈ t :=
   findP?_some_memP h
 
+@[deprecated "Use `Std.TreeMap` instead." (since := "2026-05-05")]
 theorem mem_toList_unique [Std.TransCmp (α := α) cmp] {t : RBSet α cmp}
     (hx : x ∈ toList t) (hy : y ∈ toList t) (e : cmp x y = .eq) : x = y :=
   t.2.out.1.unique (mem_toList.1 hx) (mem_toList.1 hy) e
 
+@[deprecated "Use `Std.TreeMap` instead." (since := "2026-05-05")]
 theorem findP?_some [Std.TransCmp (α := α) cmp] [IsStrictCut cmp cut] {t : RBSet α cmp} :
     t.findP? cut = some y ↔ y ∈ toList t ∧ cut y = .eq :=
   t.2.out.1.find?_some.trans <| by simp [mem_toList]
 
+@[deprecated "Use `Std.TreeMap` instead." (since := "2026-05-05")]
 theorem find?_some [Std.TransCmp (α := α) cmp] {t : RBSet α cmp} :
     t.find? x = some y ↔ y ∈ toList t ∧ cmp x y = .eq := findP?_some
 
+@[deprecated "Use `Std.TreeMap` instead." (since := "2026-05-05")]
 theorem memP_iff_findP? [Std.TransCmp (α := α) cmp] [IsCut cmp cut] {t : RBSet α cmp} :
     MemP cut t ↔ ∃ y, t.findP? cut = some y := t.2.out.1.memP_iff_find?
 
+@[deprecated "Use `Std.TreeMap` instead." (since := "2026-05-05")]
 theorem mem_iff_find? [Std.TransCmp (α := α) cmp] {t : RBSet α cmp} :
     x ∈ t ↔ ∃ y, t.find? x = some y := memP_iff_findP?
 
-@[simp] theorem contains_iff [Std.TransCmp (α := α) cmp] {t : RBSet α cmp} :
+@[deprecated "Use `Std.TreeMap` instead." (since := "2026-05-05"), simp]
+theorem contains_iff [Std.TransCmp (α := α) cmp] {t : RBSet α cmp} :
     t.contains x ↔ x ∈ t := Option.isSome_iff_exists.trans mem_iff_find?.symm
 
+@[deprecated "Use `Std.TreeMap` instead." (since := "2026-05-05")]
 instance [Std.TransCmp (α := α) cmp] {t : RBSet α cmp} : Decidable (x ∈ t) :=
   decidable_of_iff _ contains_iff
 
+@[deprecated "Use `Std.TreeMap` instead." (since := "2026-05-05")]
 theorem size_eq (t : RBSet α cmp) : t.size = t.toList.length := RBNode.size_eq
 
+@[deprecated "Use `Std.TreeMap` instead." (since := "2026-05-05")]
 theorem mem_toList_insert_self (v) (t : RBSet α cmp) : v ∈ toList (t.insert v) :=
   let ⟨_, _, h⟩ := t.2.out.2; mem_toList.2 (RBNode.mem_insert_self h)
 
+@[deprecated "Use `Std.TreeMap` instead." (since := "2026-05-05")]
 theorem mem_insert_self [Std.OrientedCmp (α := α) cmp] (v) (t : RBSet α cmp) :
     v ∈ t.insert v := mem_of_mem_toList <| mem_toList_insert_self v t
 
+@[deprecated "Use `Std.TreeMap` instead." (since := "2026-05-05")]
 theorem mem_insert_of_eq [Std.TransCmp (α := α) cmp] (t : RBSet α cmp)
     (h : cmp v v' = .eq) : v' ∈ t.insert v := (mem_congr h).1 (mem_insert_self ..)
 
+@[deprecated "Use `Std.TreeMap` instead." (since := "2026-05-05")]
 theorem mem_toList_insert_of_mem (v) {t : RBSet α cmp} (h : v' ∈ toList t) :
     v' ∈ toList (t.insert v) ∨ cmp v v' = .eq :=
   let ⟨_, _, ht⟩ := t.2.out.2
   .imp_left mem_toList.2 <| RBNode.mem_insert_of_mem ht <| mem_toList.1 h
 
+@[deprecated "Use `Std.TreeMap` instead." (since := "2026-05-05")]
 theorem mem_insert_of_mem_toList [Std.OrientedCmp (α := α) cmp] (v) {t : RBSet α cmp}
     (h : v' ∈ toList t) : v' ∈ t.insert v :=
   match mem_toList_insert_of_mem v h with
   | .inl h' => mem_of_mem_toList h'
   | .inr h' => mem_iff_mem_toList.2 ⟨_, mem_toList_insert_self .., Std.OrientedCmp.eq_comm.1 h'⟩
 
+@[deprecated "Use `Std.TreeMap` instead." (since := "2026-05-05")]
 theorem mem_insert_of_mem [Std.TransCmp (α := α) cmp] (v) {t : RBSet α cmp}
     (h : v' ∈ t) : v' ∈ t.insert v :=
   let ⟨_, h₁, h₂⟩ := mem_iff_mem_toList.1 h
   (mem_congr h₂).2 (mem_insert_of_mem_toList v h₁)
 
+@[deprecated "Use `Std.TreeMap` instead." (since := "2026-05-05")]
 theorem mem_toList_insert [Std.TransCmp (α := α) cmp] {t : RBSet α cmp} :
     v' ∈ toList (t.insert v) ↔ (v' ∈ toList t ∧ t.find? v ≠ some v') ∨ v' = v := by
   let ⟨ht₁, _, _, ht₂⟩ := t.2.out
   simpa [mem_toList] using RBNode.mem_insert ht₂ ht₁
 
+@[deprecated "Use `Std.TreeMap` instead." (since := "2026-05-05")]
 theorem mem_insert [Std.TransCmp (α := α) cmp] {t : RBSet α cmp} :
     v' ∈ t.insert v ↔ v' ∈ t ∨ cmp v v' = .eq := by
   refine ⟨fun h => ?_, fun | .inl h => mem_insert_of_mem _ h | .inr h => mem_insert_of_eq _ h⟩
@@ -958,16 +1131,20 @@ theorem mem_insert [Std.TransCmp (α := α) cmp] {t : RBSet α cmp} :
   | .inl ⟨h₃, _⟩ => exact .inl <| mem_iff_mem_toList.2 ⟨_, h₃, h₂⟩
   | .inr rfl => exact .inr <| Std.OrientedCmp.eq_comm.1 h₂
 
+@[deprecated "Use `Std.TreeMap` instead." (since := "2026-05-05")]
 theorem find?_congr [Std.TransCmp (α := α) cmp] (t : RBSet α cmp) (h : cmp v₁ v₂ = .eq) :
     t.find? v₁ = t.find? v₂ := by simp only [find?]; congr 1; funext; rw [Std.TransCmp.congr_left h]
 
+@[deprecated "Use `Std.TreeMap` instead." (since := "2026-05-05")]
 theorem findP?_insert_of_eq [Std.TransCmp (α := α) cmp] [IsStrictCut cmp cut]
     (t : RBSet α cmp) (h : cut v = .eq) : (t.insert v).findP? cut = some v :=
   findP?_some.2 ⟨mem_toList_insert_self .., h⟩
 
+@[deprecated "Use `Std.TreeMap` instead." (since := "2026-05-05")]
 theorem find?_insert_of_eq [Std.TransCmp (α := α) cmp] (t : RBSet α cmp) (h : cmp v' v = .eq) :
     (t.insert v).find? v' = some v := findP?_insert_of_eq t h
 
+@[deprecated "Use `Std.TreeMap` instead." (since := "2026-05-05")]
 theorem findP?_insert_of_ne [Std.TransCmp (α := α) cmp] [IsStrictCut cmp cut]
     (t : RBSet α cmp) (h : cut v ≠ .eq) : (t.insert v).findP? cut = t.findP? cut := by
   refine Option.ext fun u =>
@@ -976,68 +1153,88 @@ theorem findP?_insert_of_ne [Std.TransCmp (α := α) cmp] [IsStrictCut cmp cut]
   · exact mt (fun h => by rwa [IsCut.congr (cut := cut) (find?_some_eq_eq h)]) h
   · rintro rfl; contradiction
 
+@[deprecated "Use `Std.TreeMap` instead." (since := "2026-05-05")]
 theorem find?_insert_of_ne [Std.TransCmp (α := α) cmp] (t : RBSet α cmp) (h : cmp v' v ≠ .eq) :
     (t.insert v).find? v' = t.find? v' := findP?_insert_of_ne t h
 
+@[deprecated "Use `Std.TreeMap` instead." (since := "2026-05-05")]
 theorem findP?_insert [Std.TransCmp (α := α) cmp] (t : RBSet α cmp) (v cut) [IsStrictCut cmp cut] :
     (t.insert v).findP? cut = if cut v = .eq then some v else t.findP? cut := by
   split <;> [exact findP?_insert_of_eq t ‹_›; exact findP?_insert_of_ne t ‹_›]
 
+@[deprecated "Use `Std.TreeMap` instead." (since := "2026-05-05")]
 theorem find?_insert [Std.TransCmp (α := α) cmp] (t : RBSet α cmp) (v v') :
     (t.insert v).find? v' = if cmp v' v = .eq then some v else t.find? v' := findP?_insert ..
 
+@[deprecated "Use `Std.TreeMap` instead." (since := "2026-05-05")]
 theorem upperBoundP?_eq_findP? {t : RBSet α cmp} {cut} (H : t.findP? cut = some x) :
     t.upperBoundP? cut = some x := RBNode.upperBound?_eq_find? _ H
 
+@[deprecated "Use `Std.TreeMap` instead." (since := "2026-05-05")]
 theorem lowerBoundP?_eq_findP? {t : RBSet α cmp} {cut} (H : t.findP? cut = some x) :
     t.lowerBoundP? cut = some x := RBNode.lowerBound?_eq_find? _ H
 
+@[deprecated "Use `Std.TreeMap` instead." (since := "2026-05-05")]
 theorem upperBound?_eq_find? {t : RBSet α cmp} (H : t.find? x = some y) :
     t.upperBound? x = some y := upperBoundP?_eq_findP? H
 
+@[deprecated "Use `Std.TreeMap` instead." (since := "2026-05-05")]
 theorem lowerBound?_eq_find? {t : RBSet α cmp} (H : t.find? x = some y) :
     t.lowerBound? x = some y := lowerBoundP?_eq_findP? H
 
 /-- The value `x` returned by `upperBoundP?` is greater or equal to the `cut`. -/
+@[deprecated "Use `Std.TreeMap` instead." (since := "2026-05-05")]
 theorem upperBoundP?_ge {t : RBSet α cmp} : t.upperBoundP? cut = some x → cut x ≠ .gt :=
   RBNode.upperBound?_ge
 
 /-- The value `y` returned by `upperBound? x` is greater or equal to `x`. -/
+@[deprecated "Use `Std.TreeMap` instead." (since := "2026-05-05")]
 theorem upperBound?_ge {t : RBSet α cmp} : t.upperBound? x = some y → cmp x y ≠ .gt :=
   upperBoundP?_ge
 
 /-- The value `x` returned by `lowerBoundP?` is less or equal to the `cut`. -/
+@[deprecated "Use `Std.TreeMap` instead." (since := "2026-05-05")]
 theorem lowerBoundP?_le {t : RBSet α cmp} : t.lowerBoundP? cut = some x → cut x ≠ .lt :=
   RBNode.lowerBound?_le
 
 /-- The value `y` returned by `lowerBound? x` is less or equal to `x`. -/
+@[deprecated "Use `Std.TreeMap` instead." (since := "2026-05-05")]
 theorem lowerBound?_le {t : RBSet α cmp} : t.lowerBound? x = some y → cmp x y ≠ .lt :=
   lowerBoundP?_le
 
+@[deprecated "Use `Std.TreeMap` instead." (since := "2026-05-05")]
 theorem upperBoundP?_mem_toList {t : RBSet α cmp} (h : t.upperBoundP? cut = some x) :
     x ∈ t.toList := mem_toList.2 (RBNode.upperBound?_mem h)
 
+@[deprecated "Use `Std.TreeMap` instead." (since := "2026-05-05")]
 theorem upperBound?_mem_toList {t : RBSet α cmp} (h : t.upperBound? x = some y) :
     y ∈ t.toList := upperBoundP?_mem_toList h
 
+@[deprecated "Use `Std.TreeMap` instead." (since := "2026-05-05")]
 theorem lowerBoundP?_mem_toList {t : RBSet α cmp} (h : t.lowerBoundP? cut = some x) :
     x ∈ t.toList := mem_toList.2 (RBNode.lowerBound?_mem h)
 
+@[deprecated "Use `Std.TreeMap` instead." (since := "2026-05-05")]
 theorem lowerBound?_mem_toList {t : RBSet α cmp} (h : t.lowerBound? x = some y) :
     y ∈ t.toList := lowerBoundP?_mem_toList h
 
+@[deprecated "Use `Std.TreeMap` instead." (since := "2026-05-05")]
 theorem upperBoundP?_mem [Std.OrientedCmp (α := α) cmp] {t : RBSet α cmp}
     (h : t.upperBoundP? cut = some x) : x ∈ t := mem_of_mem_toList (upperBoundP?_mem_toList h)
 
+@[deprecated "Use `Std.TreeMap` instead." (since := "2026-05-05")]
 theorem lowerBoundP?_mem [Std.OrientedCmp (α := α) cmp] {t : RBSet α cmp}
     (h : t.lowerBoundP? cut = some x) : x ∈ t := mem_of_mem_toList (lowerBoundP?_mem_toList h)
 
+@[deprecated "Use `Std.TreeMap` instead." (since := "2026-05-05")]
 theorem upperBound?_mem [Std.OrientedCmp (α := α) cmp] {t : RBSet α cmp}
     (h : t.upperBound? x = some y) : y ∈ t := upperBoundP?_mem h
 
+@[deprecated "Use `Std.TreeMap` instead." (since := "2026-05-05")]
 theorem lowerBound?_mem [Std.OrientedCmp (α := α) cmp] {t : RBSet α cmp}
     (h : t.lowerBound? x = some y) : y ∈ t := lowerBoundP?_mem h
 
+@[deprecated "Use `Std.TreeMap` instead." (since := "2026-05-05")]
 theorem upperBoundP?_exists {t : RBSet α cmp} [Std.TransCmp cmp] [IsCut cmp cut] :
     (∃ x, t.upperBoundP? cut = some x) ↔ ∃ x ∈ t, cut x ≠ .gt := by
   simp [upperBoundP?, t.2.out.1.upperBound?_exists, mem_toList, mem_iff_mem_toList]
@@ -1045,6 +1242,7 @@ theorem upperBoundP?_exists {t : RBSet α cmp} [Std.TransCmp cmp] [IsCut cmp cut
     fun ⟨x, h1, h2⟩ => ⟨x, ⟨x, h1, Std.ReflCmp.compare_self⟩, h2⟩,
     fun ⟨x, ⟨y, h1, h2⟩, eq⟩ => ⟨y, h1, IsCut.congr (cut := cut) h2 ▸ eq⟩⟩
 
+@[deprecated "Use `Std.TreeMap` instead." (since := "2026-05-05")]
 theorem lowerBoundP?_exists {t : RBSet α cmp} [Std.TransCmp cmp] [IsCut cmp cut] :
     (∃ x, t.lowerBoundP? cut = some x) ↔ ∃ x ∈ t, cut x ≠ .lt := by
   simp [lowerBoundP?, t.2.out.1.lowerBound?_exists, mem_toList, mem_iff_mem_toList]
@@ -1052,9 +1250,11 @@ theorem lowerBoundP?_exists {t : RBSet α cmp} [Std.TransCmp cmp] [IsCut cmp cut
     fun ⟨x, h1, h2⟩ => ⟨x, ⟨x, h1, Std.ReflCmp.compare_self⟩, h2⟩,
     fun ⟨x, ⟨y, h1, h2⟩, eq⟩ => ⟨y, h1, IsCut.congr (cut := cut) h2 ▸ eq⟩⟩
 
+@[deprecated "Use `Std.TreeMap` instead." (since := "2026-05-05")]
 theorem upperBound?_exists {t : RBSet α cmp} [Std.TransCmp cmp] :
     (∃ y, t.upperBound? x = some y) ↔ ∃ y ∈ t, cmp x y ≠ .gt := upperBoundP?_exists
 
+@[deprecated "Use `Std.TreeMap` instead." (since := "2026-05-05")]
 theorem lowerBound?_exists {t : RBSet α cmp} [Std.TransCmp cmp] :
     (∃ y, t.lowerBound? x = some y) ↔ ∃ y ∈ t, cmp x y ≠ .lt := lowerBoundP?_exists
 
@@ -1063,6 +1263,7 @@ A statement of the least-ness of the result of `upperBoundP?`. If `x` is the ret
 `upperBoundP?` and it is strictly greater than the cut, then any other `y < x` in the tree is in
 fact strictly less than the cut (so there is no exact match, and nothing closer to the cut).
 -/
+@[deprecated "Use `Std.TreeMap` instead." (since := "2026-05-05")]
 theorem upperBoundP?_least {t : RBSet α cmp} [Std.TransCmp cmp] [IsCut cmp cut]
     (H : t.upperBoundP? cut = some x) (hy : y ∈ t)
     (xy : cmp y x = .lt) (hx : cut x = .lt) : cut y = .gt :=
@@ -1075,6 +1276,7 @@ A statement of the greatest-ness of the result of `lowerBoundP?`. If `x` is the 
 `lowerBoundP?` and it is strictly less than the cut, then any other `y > x` in the tree is in fact
 strictly greater than the cut (so there is no exact match, and nothing closer to the cut).
 -/
+@[deprecated "Use `Std.TreeMap` instead." (since := "2026-05-05")]
 theorem lowerBoundP?_greatest {t : RBSet α cmp} [Std.TransCmp cmp] [IsCut cmp cut]
     (H : t.lowerBoundP? cut = some x) (hy : y ∈ t)
     (xy : cmp x y = .lt) (hx : cut x = .gt) : cut y = .lt :=
@@ -1082,19 +1284,24 @@ theorem lowerBoundP?_greatest {t : RBSet α cmp} [Std.TransCmp cmp] [IsCut cmp c
   IsCut.congr (cut := cut) h2 ▸
   t.2.out.1.lowerBound?_greatest H (mem_toList.1 h1) (Std.TransCmp.congr_right h2 ▸ xy) hx
 
+@[deprecated "Use `Std.TreeMap` instead." (since := "2026-05-05")]
 theorem memP_iff_upperBoundP? {t : RBSet α cmp} [Std.TransCmp cmp] [IsCut cmp cut] :
     t.MemP cut ↔ ∃ x, t.upperBoundP? cut = some x ∧ cut x = .eq := t.2.out.1.memP_iff_upperBound?
 
+@[deprecated "Use `Std.TreeMap` instead." (since := "2026-05-05")]
 theorem memP_iff_lowerBoundP? {t : RBSet α cmp} [Std.TransCmp cmp] [IsCut cmp cut] :
     t.MemP cut ↔ ∃ x, t.lowerBoundP? cut = some x ∧ cut x = .eq := t.2.out.1.memP_iff_lowerBound?
 
+@[deprecated "Use `Std.TreeMap` instead." (since := "2026-05-05")]
 theorem mem_iff_upperBound? {t : RBSet α cmp} [Std.TransCmp cmp] :
     x ∈ t ↔ ∃ y, t.upperBound? x = some y ∧ cmp x y = .eq := memP_iff_upperBoundP?
 
+@[deprecated "Use `Std.TreeMap` instead." (since := "2026-05-05")]
 theorem mem_iff_lowerBound? {t : RBSet α cmp} [Std.TransCmp cmp] :
     x ∈ t ↔ ∃ y, t.lowerBound? x = some y ∧ cmp x y = .eq := memP_iff_lowerBoundP?
 
 /-- A stronger version of `upperBoundP?_least` that holds when the cut is strict. -/
+@[deprecated "Use `Std.TreeMap` instead." (since := "2026-05-05")]
 theorem lt_upperBoundP? {t : RBSet α cmp} [Std.TransCmp cmp] [IsStrictCut cmp cut]
     (H : t.upperBoundP? cut = some x) (hy : y ∈ t) : cmp y x = .lt ↔ cut y = .gt :=
   let ⟨_, h1, h2⟩ := mem_iff_mem_toList.1 hy
@@ -1102,16 +1309,19 @@ theorem lt_upperBoundP? {t : RBSet α cmp} [Std.TransCmp cmp] [IsStrictCut cmp c
   t.2.out.1.lt_upperBound? H (mem_toList.1 h1)
 
 /-- A stronger version of `lowerBoundP?_greatest` that holds when the cut is strict. -/
+@[deprecated "Use `Std.TreeMap` instead." (since := "2026-05-05")]
 theorem lowerBoundP?_lt {t : RBSet α cmp} [Std.TransCmp cmp] [IsStrictCut cmp cut]
     (H : t.lowerBoundP? cut = some x) (hy : y ∈ t) : cmp x y = .lt ↔ cut y = .lt :=
   let ⟨_, h1, h2⟩ := mem_iff_mem_toList.1 hy
   IsCut.congr (cut := cut) h2 ▸ Std.TransCmp.congr_right h2 ▸
   t.2.out.1.lowerBound?_lt H (mem_toList.1 h1)
 
+@[deprecated "Use `Std.TreeMap` instead." (since := "2026-05-05")]
 theorem lt_upperBound? {t : RBSet α cmp} [Std.TransCmp cmp]
     (H : t.upperBound? x = some y) (hz : z ∈ t) : cmp z y = .lt ↔ cmp z x = .lt :=
   (lt_upperBoundP? H hz).trans Std.OrientedCmp.gt_iff_lt
 
+@[deprecated "Use `Std.TreeMap` instead." (since := "2026-05-05")]
 theorem lowerBound?_lt {t : RBSet α cmp} [Std.TransCmp cmp]
     (H : t.lowerBound? x = some y) (hz : z ∈ t) : cmp y z = .lt ↔ cmp x z = .lt :=
   lowerBoundP?_lt H hz
@@ -1121,125 +1331,162 @@ end RBSet
 namespace RBMap
 
 -- @[simp] -- FIXME: RBSet.val_toList already triggers here, seems bad?
+@[deprecated "Use `Std.TreeMap` instead." (since := "2026-05-05")]
 theorem val_toList {t : RBMap α β cmp} : t.1.toList = t.toList := rfl
 
-@[simp] theorem mkRBSet_eq : mkRBMap α β cmp = ∅ := rfl
-@[simp] theorem empty_eq : @RBMap.empty α β cmp = ∅ := rfl
-@[simp] theorem default_eq : (default : RBMap α β cmp) = ∅ := rfl
-@[simp] theorem empty_toList : toList (∅ : RBMap α β cmp) = [] := rfl
-@[simp] theorem single_toList : toList (single a b : RBMap α β cmp) = [(a, b)] := rfl
+@[deprecated "Use `Std.TreeMap` instead." (since := "2026-05-05"), simp]
+theorem mkRBSet_eq : mkRBMap α β cmp = ∅ := rfl
+@[deprecated "Use `Std.TreeMap` instead." (since := "2026-05-05"), simp]
+theorem empty_eq : @RBMap.empty α β cmp = ∅ := rfl
+@[deprecated "Use `Std.TreeMap` instead." (since := "2026-05-05"), simp]
+theorem default_eq : (default : RBMap α β cmp) = ∅ := rfl
+@[deprecated "Use `Std.TreeMap` instead." (since := "2026-05-05"), simp]
+theorem empty_toList : toList (∅ : RBMap α β cmp) = [] := rfl
+@[deprecated "Use `Std.TreeMap` instead." (since := "2026-05-05"), simp]
+theorem single_toList : toList (single a b : RBMap α β cmp) = [(a, b)] := rfl
 
+@[deprecated "Use `Std.TreeMap` instead." (since := "2026-05-05")]
 theorem mem_toList {t : RBMap α β cmp} : x ∈ toList t ↔ x ∈ t.1 := RBNode.mem_toList
 
+@[deprecated "Use `Std.TreeMap` instead." (since := "2026-05-05")]
 theorem foldl_eq_foldl_toList {t : RBMap α β cmp} :
     t.foldl f init = t.toList.foldl (fun r p => f r p.1 p.2) init :=
   RBNode.foldl_eq_foldl_toList
 
+@[deprecated "Use `Std.TreeMap` instead." (since := "2026-05-05")]
 theorem foldr_eq_foldr_toList {t : RBMap α β cmp} :
     t.foldr f init = t.toList.foldr (fun p r => f p.1 p.2 r) init :=
   RBNode.foldr_eq_foldr_toList
 
+@[deprecated "Use `Std.TreeMap` instead." (since := "2026-05-05")]
 theorem foldlM_eq_foldlM_toList [Monad m] [LawfulMonad m] {t : RBMap α β cmp} :
     t.foldlM (m := m) f init = t.toList.foldlM (fun r p => f r p.1 p.2) init :=
   RBNode.foldlM_eq_foldlM_toList
 
+@[deprecated "Use `Std.TreeMap` instead." (since := "2026-05-05")]
 theorem forM_eq_forM_toList [Monad m] [LawfulMonad m] {t : RBMap α β cmp} :
     t.forM (m := m) f = t.toList.forM (fun p => f p.1 p.2) :=
   RBNode.forM_eq_forM_toList
 
+@[deprecated "Use `Std.TreeMap` instead." (since := "2026-05-05")]
 theorem forIn_eq_forIn_toList [Monad m] [LawfulMonad m] {t : RBMap α β cmp} :
     forIn (m := m) t init f = forIn t.toList init f := RBNode.forIn_eq_forIn_toList
 
+@[deprecated "Use `Std.TreeMap` instead." (since := "2026-05-05")]
 theorem toStream_eq {t : RBMap α β cmp} : Std.toStream t = t.1.toStream .nil := rfl
 
-@[simp] theorem toStream_toList {t : RBMap α β cmp} : (Std.toStream t).toList = t.toList :=
+@[deprecated "Use `Std.TreeMap` instead." (since := "2026-05-05"), simp]
+theorem toStream_toList {t : RBMap α β cmp} : (Std.toStream t).toList = t.toList :=
   RBSet.toStream_toList
 
+@[deprecated "Use `Std.TreeMap` instead." (since := "2026-05-05")]
 theorem toList_sorted {t : RBMap α β cmp} : t.toList.Pairwise (RBNode.cmpLT (cmp ·.1 ·.1)) :=
   RBSet.toList_sorted
 
+@[deprecated "Use `Std.TreeMap` instead." (since := "2026-05-05")]
 theorem findEntry?_some_eq_eq {t : RBMap α β cmp} : t.findEntry? x = some (y, v) → cmp x y = .eq :=
   RBSet.findP?_some_eq_eq
 
+@[deprecated "Use `Std.TreeMap` instead." (since := "2026-05-05")]
 theorem findEntry?_some_mem_toList {t : RBMap α β cmp} (h : t.findEntry? x = some y) :
     y ∈ toList t := RBSet.findP?_some_mem_toList h
 
+@[deprecated "Use `Std.TreeMap` instead." (since := "2026-05-05")]
 theorem find?_some_mem_toList {t : RBMap α β cmp} (h : t.find? x = some v) :
     ∃ y, (y, v) ∈ toList t ∧ cmp x y = .eq := by
   obtain ⟨⟨y, v⟩, h', rfl⟩ := Option.map_eq_some_iff.1 h
   exact ⟨_, findEntry?_some_mem_toList h', findEntry?_some_eq_eq h'⟩
 
+@[deprecated "Use `Std.TreeMap` instead." (since := "2026-05-05")]
 theorem mem_toList_unique [Std.TransCmp (α := α) cmp] {t : RBMap α β cmp}
     (hx : x ∈ toList t) (hy : y ∈ toList t) (e : cmp x.1 y.1 = .eq) : x = y :=
   RBSet.mem_toList_unique hx hy e
 
 /-- A "representable cut" is one generated by `cmp a` for some `a`. This is always a valid cut. -/
+@[deprecated "Use `Std.TreeMap` instead." (since := "2026-05-05")]
 instance (cmp) (a : α) : IsStrictCut cmp (cmp a) where
   le_lt_trans h₁ h₂ := Std.TransCmp.lt_of_lt_of_le h₂ h₁
   le_gt_trans h₁ := Decidable.not_imp_not.1 (Std.TransCmp.le_trans · h₁)
   exact h := (Std.TransCmp.congr_left h).symm
 
+@[deprecated "Use `Std.TreeMap` instead." (since := "2026-05-05")]
 instance (f : α → β) (cmp) [Std.TransCmp (α := β) cmp] (x : β) :
     IsStrictCut (Ordering.byKey f cmp) (fun y => cmp x (f y)) where
   le_lt_trans h₁ h₂ := Std.TransCmp.lt_of_lt_of_le h₂ h₁
   le_gt_trans h₁ := Decidable.not_imp_not.1 (Std.TransCmp.le_trans · h₁)
   exact h := (Std.TransCmp.congr_left h).symm
 
+@[deprecated "Use `Std.TreeMap` instead." (since := "2026-05-05")]
 theorem findEntry?_some [Std.TransCmp (α := α) cmp] {t : RBMap α β cmp} :
     t.findEntry? x = some y ↔ y ∈ toList t ∧ cmp x y.1 = .eq := RBSet.findP?_some
 
+@[deprecated "Use `Std.TreeMap` instead." (since := "2026-05-05")]
 theorem find?_some [Std.TransCmp (α := α) cmp] {t : RBMap α β cmp} :
     t.find? x = some v ↔ ∃ y, (y, v) ∈ toList t ∧ cmp x y = .eq := by
   simp only [find?, findEntry?_some, Option.map_eq_some_iff]; constructor
   · rintro ⟨_, h, rfl⟩; exact ⟨_, h⟩
   · rintro ⟨b, h⟩; exact ⟨_, h, rfl⟩
 
+@[deprecated "Use `Std.TreeMap` instead." (since := "2026-05-05")]
 theorem contains_iff_findEntry? {t : RBMap α β cmp} :
     t.contains x ↔ ∃ v, t.findEntry? x = some v := Option.isSome_iff_exists
 
+@[deprecated "Use `Std.TreeMap` instead." (since := "2026-05-05")]
 theorem contains_iff_find? {t : RBMap α β cmp} :
     t.contains x ↔ ∃ v, t.find? x = some v := by
   simp only [contains_iff_findEntry?, Prod.exists, find?, Option.map_eq_some_iff, and_comm,
     exists_eq_left]
   rw [exists_comm]
 
+@[deprecated "Use `Std.TreeMap` instead." (since := "2026-05-05")]
 theorem size_eq (t : RBMap α β cmp) : t.size = t.toList.length := RBNode.size_eq
 
+@[deprecated "Use `Std.TreeMap` instead." (since := "2026-05-05")]
 theorem mem_toList_insert_self (v) (t : RBMap α β cmp) : (k, v) ∈ toList (t.insert k v) :=
   RBSet.mem_toList_insert_self ..
 
+@[deprecated "Use `Std.TreeMap` instead." (since := "2026-05-05")]
 theorem mem_toList_insert_of_mem (v) {t : RBMap α β cmp} (h : y ∈ toList t) :
     y ∈ toList (t.insert k v) ∨ cmp k y.1 = .eq := RBSet.mem_toList_insert_of_mem _ h
 
+@[deprecated "Use `Std.TreeMap` instead." (since := "2026-05-05")]
 theorem mem_toList_insert [Std.TransCmp (α := α) cmp] {t : RBMap α β cmp} :
     y ∈ toList (t.insert k v) ↔ (y ∈ toList t ∧ t.findEntry? k ≠ some y) ∨ y = (k, v) :=
   RBSet.mem_toList_insert
 
+@[deprecated "Use `Std.TreeMap` instead." (since := "2026-05-05")]
 theorem findEntry?_congr [Std.TransCmp (α := α) cmp] (t : RBMap α β cmp) (h : cmp k₁ k₂ = .eq) :
     t.findEntry? k₁ = t.findEntry? k₂ := by
   simp only [findEntry?]; congr; funext; rw [Std.TransCmp.congr_left h]
 
+@[deprecated "Use `Std.TreeMap` instead." (since := "2026-05-05")]
 theorem find?_congr [Std.TransCmp (α := α) cmp] (t : RBMap α β cmp) (h : cmp k₁ k₂ = .eq) :
     t.find? k₁ = t.find? k₂ := by simp [find?, findEntry?_congr _ h]
 
+@[deprecated "Use `Std.TreeMap` instead." (since := "2026-05-05")]
 theorem findEntry?_insert_of_eq [Std.TransCmp (α := α) cmp] (t : RBMap α β cmp)
     (h : cmp k' k = .eq) : (t.insert k v).findEntry? k' = some (k, v) :=
   RBSet.findP?_insert_of_eq _ h
 
+@[deprecated "Use `Std.TreeMap` instead." (since := "2026-05-05")]
 theorem find?_insert_of_eq [Std.TransCmp (α := α) cmp] (t : RBMap α β cmp) (h : cmp k' k = .eq) :
     (t.insert k v).find? k' = some v := by rw [find?, findEntry?_insert_of_eq _ h]; rfl
 
+@[deprecated "Use `Std.TreeMap` instead." (since := "2026-05-05")]
 theorem findEntry?_insert_of_ne [Std.TransCmp (α := α) cmp] (t : RBMap α β cmp)
     (h : cmp k' k ≠ .eq) : (t.insert k v).findEntry? k' = t.findEntry? k' :=
   RBSet.findP?_insert_of_ne _ h
 
+@[deprecated "Use `Std.TreeMap` instead." (since := "2026-05-05")]
 theorem find?_insert_of_ne [Std.TransCmp (α := α) cmp] (t : RBMap α β cmp) (h : cmp k' k ≠ .eq) :
     (t.insert k v).find? k' = t.find? k' := by simp [find?, findEntry?_insert_of_ne _ h]
 
+@[deprecated "Use `Std.TreeMap` instead." (since := "2026-05-05")]
 theorem findEntry?_insert [Std.TransCmp (α := α) cmp] (t : RBMap α β cmp) (k v k') :
     (t.insert k v).findEntry? k' = if cmp k' k = .eq then some (k, v) else t.findEntry? k' :=
   RBSet.findP?_insert ..
 
+@[deprecated "Use `Std.TreeMap` instead." (since := "2026-05-05")]
 theorem find?_insert [Std.TransCmp (α := α) cmp] (t : RBMap α β cmp) (k v k') :
     (t.insert k v).find? k' = if cmp k' k = .eq then some v else t.find? k' := by
   split <;> [exact find?_insert_of_eq t ‹_›; exact find?_insert_of_ne t ‹_›]
